store/impl.v
@@ -7,6 +7,7 @@ From iris.heap_lang Require Import notation proofmode.
 From iris.heap_lang.lib Require Import lock ticket_lock.
 From cryptis Require Import lib version term cryptis primitives tactics.
 From cryptis Require Import role session pk_auth pk_dh.
+From cryptis.store Require Import alist db.
 
 Set Implicit Arguments.
 Unset Strict Implicit.
@@ -15,11 +16,23 @@ Unset Printing Implicit Defensive.
 Record cst := {
   cst_ts   : loc;
   cst_key  : term;
+  cst_name : gname;
   cst_ok   : bool;
 }.
 
 #[global]
 Instance cst_repr : Repr cst := λ s, (#(cst_ts s), Spec.mkskey (cst_key s))%V.
+
+Record sst := {
+  sst_ts  : loc;
+  sst_key : term;
+  sst_db  : loc;
+  sst_ok  : bool;
+}.
+
+#[global]
+Instance sst_repr : Repr sst :=
+  λ s, (#(sst_ts s), Spec.mkskey (sst_key s), #(sst_db s))%V.
 
 (* FIXME: Maybe generalize this *)
 Definition sess_recv N : val := λ: "c" "k" "f",
@@ -37,51 +50,52 @@ Variable N : namespace.
 
 Definition connect : val := λ: "c" "skA" "pkA" "pkB",
   do_until (λ: <>,
-    bind: "kS" := pk_dh_init N "c" "skA" "pkA" "pkB" in
-    let: "l"  := ref #0 in
-    let: "kS" := mkskey (tag (nroot.@"keys".@"sym") "kS") in
-    send "c" (tsenc (N.@"init") "kS" (TInt 0));;
-    SOME ("l", "kS")
+    bind: "session_key" := pk_dh_init N "c" "skA" "pkA" "pkB" in
+    let: "timestamp"  := ref #0 in
+    let: "session_key" := mkskey (tag (nroot.@"keys".@"sym") "session_key") in
+    send "c" (tsenc (N.@"init") "session_key" (TInt 0));;
+    SOME ("timestamp", "session_key")
   ).
 
-Definition get_ts : val := λ: "cs",
-  let: "l" := Fst "cs" in
-  !"l".
+Definition get_timestamp : val := λ: "cs",
+  let: "timestamp" := Fst "cs" in
+  !"timestamp".
 
-Definition next_ts : val := λ: "cs",
-  let: "l" := Fst "cs" in
-  "l" <- (!"l" + #1).
+Definition incr_timestamp : val := λ: "cs",
+  let: "timestamp" := Fst "cs" in
+  "timestamp" <- (!"timestamp" + #1).
 
-Definition get_sk : val := λ: "cs",
+Definition get_session_key : val := λ: "cs",
   Snd "cs".
 
-Definition send_store : val := λ: "c" "cs" "v",
-  next_ts "cs";;
-  let: "n" := get_ts "cs" in
-  let: "sk" := get_sk "cs" in
-  let: "m" := tsenc (N.@"store") "sk" (term_of_list [tint "n"; "v"]) in
+Definition send_store : val := λ: "c" "cs" "k" "v",
+  let: "ts" := get_timestamp "cs" in
+  incr_timestamp "cs";;
+  let: "sk" := get_session_key "cs" in
+  let: "m" := tsenc (N.@"store") "sk" (term_of_list [tint "ts"; "k"; "v"]) in
   send "c" "m".
 
 Definition ack_store : val := λ: "c" "cs",
-  let: "n" := get_ts "cs" in
-  let: "sk" := get_sk "cs" in
+  let: "ts" := get_timestamp "cs" in
+  let: "sk" := get_session_key "cs" in
   sess_recv (N.@"ack_store") "c" "sk" (λ: "m",
-    assert: eq_term "m" (tint "n") in
+    assert: eq_term "m" (tint "ts") in
     SOME #()
   ).
 
-Definition store : val := λ: "c" "cs" "t",
-  send_store "c" "cs" "t";;
+Definition store : val := λ: "c" "cs" "k" "v",
+  send_store "c" "cs" "k" "v";;
   ack_store "c" "cs".
 
-Definition load : val := λ: "c" "cs",
-  let: "n" := tint (get_ts "cs") in
-  let: "sk" := get_sk "cs" in
-  send "c" (tsenc (N.@"load") "sk" "n");;
+Definition load : val := λ: "c" "cs" "k",
+  let: "ts" := tint (get_timestamp "cs") in
+  let: "sk" := get_session_key "cs" in
+  send "c" (tsenc (N.@"load") "sk" (term_of_list ["ts"; "k"]));;
   sess_recv (N.@"ack_load") "c" "sk" (λ: "resp",
     bind: "resp" := list_of_term "resp" in
-    list_match: ["n'"; "t"] := "resp" in
-    assert: eq_term "n'" "n" in
+    list_match: ["ts'"; "k'"; "t"] := "resp" in
+    assert: eq_term "ts'" "ts" in
+    assert: eq_term "k'" "k" in
     SOME "t"
   ).
 
@@ -89,77 +103,73 @@ End Client.
 
 End Client.
 
-Record sst := {
-  sst_ts   : loc;
-  sst_val  : loc;
-  sst_key  : term;
-  sst_ok   : bool;
-}.
-
-#[global]
-Instance sst_repr : Repr sst :=
-  λ ss, (#(sst_ts ss), #(sst_val ss), Spec.mkskey (sst_key ss))%V.
-
 Module Server.
 
 Implicit Types N : namespace.
 
-Definition get_ts : val := λ: "ss",
-  !(Fst (Fst "ss")).
+Definition handle_store N : val :=
+λ: "c" "ss" "req",
+  let: "timestamp" := Fst (Fst "ss") in
+  let: "session_key" := Snd (Fst "ss") in
+  let: "db" := Snd "ss" in
+  bind: "req" := tsdec (N.@"store") "session_key" "req" in
+  bind: "req" := list_of_term "req" in
+  list_match: ["timestamp'"; "k"; "v"] := "req" in
+  bind: "timestamp'" := to_int "timestamp'" in
+  assert: !"timestamp" = "timestamp'" in
+  "timestamp" <- !"timestamp" + #1;;
+  "db" <- AList.insert !"db" "k" "v";;
+  send "c" (tsenc (N.@"ack_store") "session_key" (tint "timestamp'"));;
+  SOME #().
 
-Definition get_val : val := λ: "ss",
-  !(Snd (Fst "ss")).
+Definition handle_load N : val :=
+λ: "c" "ss" "req",
+  let: "timestamp" := ! (Fst (Fst "ss")) in
+  let: "session_key" := Snd (Fst "ss") in
+  let: "db" := ! (Snd "ss") in
+  bind: "req" := tsdec (N.@"load") "session_key" "req" in
+  bind: "req" := list_of_term "req" in
+  list_match: ["timestamp'"; "k"] := "req" in
+  bind: "timestamp'" := to_int "timestamp'" in
+  assert: "timestamp" = "timestamp'" in
+  bind: "data" := AList.find "db" "k" in
+  let: "m" := term_of_list [ tint "timestamp"; "k"; "data"] in
+  send "c" (tsenc (N.@"ack_load") "session_key" "m");;
+  SOME #().
 
-Definition upd_val : val := λ: "ss" "ts" "v",
-  Fst (Fst "ss") <- "ts" ;;
-  Snd (Fst "ss") <- "v".
-
-Definition get_key : val := λ: "ss",
-  Snd "ss".
-
-Definition handle_store N : val := λ: "c" "ss" "m",
-  bind: "m" := list_of_term "m" in
-  list_match: ["n"; "x"] := "m" in
-  bind: "n'" := to_int "n" in
-  assert: get_ts "ss" ≤ "n'" in
-  upd_val "ss" "n'" "x";;
-  send "c" (tsenc (N.@"ack_store") (get_key "ss") "n").
-
-Definition handle_load N : val := λ: "c" "ss" "m",
-  bind: "n" := to_int "m" in
-  assert: get_ts "ss" = "n" in
-  let: "v" := get_val "ss" in
-  send "c" (tsenc (N.@"ack_load") (get_key "ss") (term_of_list ["m"; "v"])).
-
-Definition conn_handler_body N : val := λ: "c" "ss",
-  let: "sk" := get_key "ss" in
+Definition conn_handler_body N : val :=
+λ: "c" "ss",
   let: "m" := recv "c" in
-  match: tsdec (N.@"store") "sk" "m" with
-    SOME "m" => handle_store N "c" "ss" "m"
-  | NONE => match: tsdec (N.@"load") "sk" "m" with
-    SOME "m" => handle_load N "c" "ss" "m"
+  match: handle_store N "c" "ss" "m" with
+    SOME <> => #()
+  | NONE => match: handle_load N "c" "ss" "m" with
+    SOME <> => #()
   | NONE => #()
   end end.
 
-Definition conn_handler N : val := rec: "loop" "c" "ss" :=
+Definition conn_handler N : val :=
+rec: "loop" "c" "ss" :=
   conn_handler_body N "c" "ss";;
   "loop" "c" "ss".
 
-Definition wait_init N : val := λ: "c" "kS",
-  sess_recv (N.@"init") "c" "kS" (λ: <>,
-    let: "ss" := (ref #0, ref (TInt 0), "kS") in
-    conn_handler N "c" "ss"
+Definition wait_init N : val :=
+  λ: "c" "session_key",
+  sess_recv (N.@"init") "c" "session_key" (λ: <>,
+    let: "db" := ref (AList.empty #()) in
+    conn_handler N "c" (ref #0, "session_key", "db")
   ).
 
-Definition listen N : val := rec: "loop" "c" "skB" "pkB" :=
-  match: pk_dh_resp N "c" "skB" "pkB" with
+Definition listen N : val :=
+rec: "loop" "c" "secret_key" "public_key" :=
+  match: pk_dh_resp N "c" "secret_key" "public_key" with
     NONE =>
-    "loop" "c" "skB" "pkB"
+    "loop" "c" "secret_key" "public_key"
   | SOME "res" =>
-    let: "pkA" := Fst "res" in (* Unused for now *)
-    let: "kS"  := mkskey (tag (nroot.@"keys".@"sym") (Snd "res")) in
-    Fork (wait_init N "c" "kS");;
-    "loop" "c" "skB" "pkB"
+    (* Unused for now *)
+    let: "client_key" := Fst "res" in
+    let: "session_key"  := mkskey (tag (nroot.@"keys".@"sym") (Snd "res")) in
+    Fork (wait_init N "c" "session_key");;
+    "loop" "c" "secret_key" "public_key"
   end.
 
 End Server.
