store/server_proofs.v
@@ -6,7 +6,7 @@ From iris.algebra Require Import max_prefix_list.
 From iris.heap_lang Require Import notation proofmode.
 From cryptis Require Import lib version term cryptis primitives tactics.
 From cryptis Require Import role session pk_auth pk_dh.
-From cryptis.store Require Import impl shared.
+From cryptis.store Require Import impl shared alist db.
 
 Set Implicit Arguments.
 Unset Strict Implicit.
@@ -17,7 +17,7 @@ Section Verif.
 Context `{!cryptisGS Σ, !heapGS Σ, !sessionGS Σ}.
 Notation iProp := (iProp Σ).
 
-Context `{!storeG Σ}.
+Context `{!storeGS Σ}.
 
 Local Instance STORE : PK := PK_DH (λ _ _ _ _, True)%I.
 
@@ -28,67 +28,6 @@ Implicit Types γ : gname.
 Implicit Types v : val.
 
 Variable N : namespace.
-
-Definition server_state s n t : iProp :=
-  sst_ts s ↦ #n ∗
-  sst_val s ↦ repr t ∗
-  minted (sst_key s) ∗
-  public t ∗
-  handshake_done N (sst_key s) (sst_ok s) ∗
-  if sst_ok s then value_frag N (sst_key s) n t else True%I.
-
-Lemma server_state_frag s n t :
-  server_state s n t -∗
-  minted (sst_key s) ∗
-  public t ∗
-  handshake_done N (sst_key s) (sst_ok s) ∗
-  if sst_ok s then value_frag N (sst_key s) n t else True%I.
-Proof. by iIntros "(_ & _ & ?)". Qed.
-
-Lemma wp_server_get_ts E ss n t :
-  {{{ server_state ss n t }}}
-    Server.get_ts (repr ss) @ E
-  {{{ RET #n; server_state ss n t }}}.
-Proof.
-iIntros "%Φ (ts & val & ?) post".
-rewrite /Server.get_ts. wp_pures. wp_load. iApply "post".
-by iFrame.
-Qed.
-
-Lemma wp_server_upd_val E ss n t n' t' :
-  {{{ ▷ server_state ss n t ∗
-      ▷ public t' ∗
-      ▷ if sst_ok ss then value_frag N (sst_key ss) n' t' else True%I }}}
-    Server.upd_val (repr ss) #n' t' @ E
-  {{{ RET #(); server_state ss n' t' }}}.
-Proof.
-iIntros "%Φ ((ts & val & ? & ? & #frag & key) & p_t' & #frag') post".
-rewrite /Server.upd_val. wp_pures. wp_store. wp_pures. wp_store.
-iApply "post". iFrame. by eauto.
-Qed.
-
-Lemma wp_server_get_val E ss n t :
-  {{{ server_state ss n t }}}
-    Server.get_val (repr ss) @ E
-  {{{ RET (repr t);
-      public t ∗
-      (if sst_ok ss then value_frag N (sst_key ss) n t else True%I) ∗
-      server_state ss n t }}}.
-Proof.
-iIntros "%Φ (ts & val & ? & #? & #done & #frag) post".
-rewrite /Server.get_val. wp_pures. wp_load. iApply "post".
-iFrame. iModIntro. by eauto.
-Qed.
-
-Lemma wp_server_get_key E ss n t :
-  {{{ server_state ss n t }}}
-    Server.get_key (repr ss) @ E
-  {{{ RET (repr (Spec.mkskey (sst_key ss)));
-      server_state ss n t }}}.
-Proof.
-iIntros "%Φ ? post".
-rewrite /Server.get_key. wp_pures. by iApply "post".
-Qed.
 
 Lemma ack_storeI kS n :
   store_ctx N -∗
@@ -103,124 +42,134 @@ iApply public_TEncIS => //.
 - by rewrite public_TInt; eauto.
 Qed.
 
-Lemma wp_server_handle_store E c ss n t m :
+Lemma wp_server_handle_store E c ss m :
   ↑cryptisN ⊆ E →
   channel c -∗
   store_ctx N -∗
-  public (TEnc (sst_key ss) (Spec.tag (N.@"store") m)) -∗
-  {{{ server_state ss n t }}}
+  public m -∗
+  {{{ server N ss }}}
     Server.handle_store N c (repr ss) m @ E
-  {{{ n' t' v, RET v; server_state ss n' t' }}}.
+  {{{ (v : option val), RET (repr v); server N ss }}}.
 Proof.
 iIntros "%sub #chan_c #ctx #p_m !> %Φ state post".
 rewrite /Server.handle_store. wp_pures.
-wp_list_of_term m; wp_pures; last by iApply "post".
-wp_list_match => [n' t' ->|_]; wp_pures; last by iApply "post".
+wp_tsdec m; wp_pures; last by iApply ("post" $! None).
+wp_list_of_term m; wp_pures; last by iApply ("post" $! None).
+wp_list_match => [n' t1 t2 ->|_]; wp_pures; last by iApply ("post" $! None).
 wp_bind (to_int _). iApply wp_to_int.
-case: Spec.to_intP => [ {}n' -> | _]; wp_pures; last by iApply "post".
-wp_bind (Server.get_ts _). iApply (wp_server_get_ts with "state").
-iIntros "!> state". wp_pures.
-case: bool_decide_reflect => [nn'|_]; wp_pures; last by iApply "post".
-have {n' nn'} [n' ->] : ∃ n'' : nat, n' = n''.
-  exists (Z.to_nat n'). by lia.
-iPoseProof (server_state_frag with "state") as "#(_ & _ & done & frag)".
-iAssert (if sst_ok ss then ∃ γ, wf_key N (sst_key ss) γ else True)%I
-  as "{frag} #frag".
+case: Spec.to_intP => [ {}n' -> | _]; wp_pures; last by iApply ("post" $! None).
+iDestruct "state" as "(%n & %kvs & %db & #handshake & #minted_key & ts & 
+                       db & %kvs_db & #pub_db & view)".
+wp_load. wp_pures.
+case: bool_decide_reflect => [[<-]|ne]; wp_pures; last first.
+{ iModIntro. iApply ("post" $! None).
+  iExists n, kvs, db. iFrame. by eauto. }
+wp_load. wp_pures.
+replace (n + 1)%Z with (S n : Z) by lia.
+wp_store. wp_load. wp_bind (AList.insert _ _ _).
+wp_pures. iApply AList.wp_insert; eauto. iIntros "!> %kvs' %kvs'_db'".
+iDestruct (store_predE with "handshake [#] [//] p_m") as "(p_t1 & p_t2 & wf')".
 { case: sst_ok => //.
-  by iDestruct "frag" as "(% & _ & ?)"; eauto. }
-iPoseProof (store_predE with "done frag ctx p_m") as "(#p_t' & #frag')".
-wp_bind (Server.upd_val _ _ _).
-iApply (wp_server_upd_val with "[$]").
-iIntros "!> state". wp_pures.
-wp_bind (Server.get_key _).
-iApply (wp_server_get_key with "[$]") => //.
-iIntros "!> state". wp_tsenc. rewrite /=.
-iApply wp_send => //.
-  iModIntro. iApply ack_storeI => //.
-  iPoseProof (public_minted with "p_m") as "s_m".
-  rewrite minted_TEnc. by iDestruct "s_m" as "[??]".
-iApply "post". by eauto.
+  iDestruct "view" as "(%γ & ? & ?)". eauto. }
+wp_store. wp_bind (tint _). iApply wp_tint.
+wp_tsenc.
+iApply wp_fupd.
+wp_bind (send _ _). iApply wp_send => //.
+{ iModIntro. iApply ack_storeI => //. }
+wp_pures. iApply ("post" $! (Some #())).
+iExists (S n), kvs', (<[t1 := t2]>db). iFrame.
+do 4!iSplitR => //.
+{ iModIntro. iApply big_sepM_insert_2 => //. eauto. }
+case: sst_ok; eauto.
+iDestruct "wf'" as "(%γ1 & wf1 & update)".
+iDestruct "view" as "(%γ2 & #wf2 & #view)".
+iPoseProof (wf_key_agree with "handshake wf1 wf2") as "<-".
+iPoseProof (DB.update_server with "view update") as "view'".
+iModIntro. iExists γ1. iSplit => //.
 Qed.
 
-Lemma wp_server_handle_load E c ss n t m :
+Lemma wp_server_handle_load E c ss m :
   ↑cryptisN ⊆ E →
   channel c -∗
   store_ctx N -∗
-  public (TEnc (sst_key ss) (Spec.tag (N.@"load") m)) -∗
-  {{{ server_state ss n t }}}
+  public m -∗
+  {{{ server N ss }}}
     Server.handle_load N c (repr ss) m @ E
-  {{{ v, RET v; server_state ss n t }}}.
+  {{{ (v : option val), RET (repr v); server N ss }}}.
 Proof.
 iIntros "%sub #chan_c #ctx #p_m !> %Φ state post".
 rewrite /Server.handle_load. wp_pures.
+iDestruct "state" as "(%n & %kvs & %db & #handshake & #minted_key & ts &
+                       db & %kvs_db & #pub_db & #view)".
+wp_load. wp_pures. wp_load. wp_pures.
+iAssert (server N ss) with "[ts db view]" as "state".
+{ iExists n, kvs, db. iFrame. eauto. }
+wp_tsdec m; wp_pures; last by iApply ("post" $! None).
+wp_list_of_term m; wp_pures; last by iApply ("post" $! None).
+wp_list_match => [timestamp t1 ->| _]; wp_pures; last by iApply ("post" $! None).
 wp_bind (to_int _). iApply wp_to_int.
-case: Spec.to_intP => [ {m} n' -> | _]; wp_pures; last by iApply "post".
-wp_bind (Server.get_ts _). iApply (wp_server_get_ts with "[$]").
-iIntros "!> state". wp_pures.
-case: bool_decide_reflect => [[ {n'} <-]| _]; wp_pures; last by iApply "post".
-wp_bind (Server.get_val _). iApply (wp_server_get_val with "[$]").
-iIntros "!> (#p_t & #frag & state)". wp_pures.
-wp_list. wp_term_of_list. wp_bind (Server.get_key _).
-iApply (wp_server_get_key with "[$]").
-iIntros "!> state". wp_tsenc. rewrite /=.
-iApply (wp_send with "[//] [#]") => //; last by iApply "post".
+case: Spec.to_intP => [ {m} n' -> | _]; wp_pures; last by iApply ("post" $! None).
+case: bool_decide_reflect => [[<-]|?]; wp_pures; last by iApply ("post" $! None).
+wp_bind (AList.find _ _). iApply AList.wp_find => //.
+iIntros "!> _".
+case db_t1: (db !! t1) => [t2|]; wp_pures; last by iApply ("post" $! None).
+wp_list. wp_bind (tint _). iApply wp_tint. wp_list. wp_term_of_list.
+wp_pures. wp_tsenc. wp_bind (send _ _).
+iApply (wp_send with "[//] [#]") => //; last by wp_pures;
+  iApply ("post" $! (Some #())).
 iDestruct "ctx" as "(_ & _ & _ & _ & ? & _)".
-iDestruct "state" as "(_ & _ & #? & _ & #frag' & #key)".
-iModIntro. iApply public_TEncIS => //.
+iModIntro.
+rewrite big_sepM_delete //. iDestruct "pub_db" as "[[? ?] _]".
+iApply public_TEncIS => //.
 - rewrite minted_TKey.
   iPoseProof (public_minted with "p_m") as "{p_m} p_m".
   by rewrite minted_TEnc; iDestruct "p_m" as "[??]".
-- iModIntro.
-  iExists n, t, (sst_ok ss).
-  by eauto.
-- rewrite minted_of_list /= minted_TInt -[minted t]public_minted; eauto.
+- iModIntro. iExists n, (sst_ok ss), t1, t2. iSplit => //.
+  do 2!iSplit => //.
+  case: sst_ok => //.
+  iDestruct "view" as "(%γ & key & view)".
+  iExists γ. iSplit => //. iApply DB.load_server; eauto.
+- rewrite minted_of_list /= minted_TInt -[minted t1]public_minted.
+  rewrite -[minted t2]public_minted; eauto.
 - iIntros "!> _". by rewrite public_of_list /= public_TInt; eauto.
 Qed.
 
-Lemma wp_server_conn_handler_body E c ss n t :
+Lemma wp_server_conn_handler_body E c ss :
   ↑cryptisN ⊆ E →
   channel c -∗
   store_ctx N -∗
-  {{{ server_state ss n t }}}
+  {{{ server N ss }}}
     Server.conn_handler_body N c (repr ss) @ E
-  {{{ n' t' v, RET v; server_state ss n' t' }}}.
+  {{{ v, RET v; server N ss }}}.
 Proof.
 iIntros "% #chan_c #ctx !> %Φ state post". rewrite /Server.conn_handler_body.
-wp_pures. wp_bind (Server.get_key _).
-iApply (wp_server_get_key with "[$]"). iIntros "!> state".
 wp_pures. wp_bind (recv _). iApply wp_recv => //.
 iIntros "%m #p_m". wp_pures.
-wp_tsdec m; wp_pures; last wp_tsdec m; wp_pures; last by iApply "post".
-- iApply (wp_server_handle_store with "[# //] [# //] [# //] [$] [$]") => //.
-- iApply (wp_server_handle_load with "[# //] [# //] [# //] [$]") => //.
+wp_bind (Server.handle_store _ _ _ _).
+iApply (wp_server_handle_store with "chan_c ctx p_m state") => //.
+iIntros "!> %res state".
+case: res => [?|] /=; wp_pures; first by iApply "post".
+wp_bind (Server.handle_load _ _ _ _).
+iApply (wp_server_handle_load with "chan_c ctx p_m state") => //.
+iIntros "!> %res state".
+case: res => [?|] /=; wp_pures; first by iApply "post".
+by iApply "post".
 Qed.
 
-Lemma wp_server_conn_handler E c ss n t :
+Lemma wp_server_conn_handler E c ss :
   ↑cryptisN ⊆ E →
   channel c -∗
   store_ctx N -∗
-  {{{ server_state ss n t }}}
+  {{{ server N ss }}}
     Server.conn_handler N c (repr ss) @ E
   {{{ v, RET v; False }}}.
 Proof.
 iIntros "% #chan_c #ctx".
-iLöb as "IH" forall (n t). iIntros "!> %Φ state post". wp_rec.
+iLöb as "IH". iIntros "!> %Φ state post". wp_rec.
 wp_pures. wp_bind (Server.conn_handler_body _ _ _).
 iApply (wp_server_conn_handler_body with "[# //] [# //] [$]") => //.
-iIntros "!> %n' %t' %v state". wp_pures.
+iIntros "!> %n' state". wp_pures.
 by iApply ("IH" with "[$]").
-Qed.
-
-Lemma initE kS t :
-  store_ctx N -∗
-  public (TEnc kS (Spec.tag (N.@"init") t)) -∗
-  public (TKey Enc kS) ∨
-  ▷ ∃ ok, handshake_done N kS ok ∗
-            (if ok then value_frag N kS 0 (TInt 0) else True)%I.
-Proof.
-iIntros "(#initP & _) #p_t".
-iDestruct (public_TEncE with "[//] [//]") as "[[??]|#tP]"; first by eauto.
-iRight. by iDestruct "tP" as "(#init & _ & _)".
 Qed.
 
 Lemma wp_server_listen E c kR dq ph T :
@@ -249,26 +198,33 @@ iClear "IH". iModIntro. rewrite /Server.wait_init. wp_pures.
 iRevert "key". iApply wp_sess_recv => //.
   by rewrite minted_tag.
 iIntros "!> %t key #p_t".
-wp_pures. wp_alloc v as "Hv". wp_alloc ts as "Hts".
-pose (ss := {| sst_ts := ts; sst_val := v;
+wp_pures. wp_bind (AList.empty _).
+iApply AList.wp_empty => //. iIntros "!> %kvs %kvs0".
+wp_alloc ldb as "Hdb". wp_pures.
+wp_alloc ts as "Hts".
+iDestruct (initE with "[//] p_t") as "{p_t} p_t".
+pose (ss := {| sst_ts := ts;
                sst_key := Spec.tag (nroot.@"keys".@"sym") kS;
+               sst_db := ldb;
                sst_ok := in_honest kI kR T |}).
 iAssert (handshake_done N (sst_key ss) (sst_ok ss)) as "#done".
 { iExists kI, kR, kS, ph, T; eauto. }
-iAssert (▷ server_state ss 0 (TInt 0))%I with "[Hts Hv key]" as "state".
-{ iFrame.
-  rewrite /= minted_tag public_TInt. do 3!iSplit => //.
+iAssert (▷ server N ss)%I with "[Hts Hdb key]" as "state".
+{ iExists 0, kvs, ∅. iFrame.
+  rewrite minted_tag /= big_sepM_empty.
+  do 4!iSplitR => //.
   case e_ok: in_honest => //.
   iDestruct "key" as "(#sec & _ & #key)".
   iAssert (∀ kt, public (TKey kt (sst_key ss)) -∗ ◇ False)%I as "{sec} sec".
   { iIntros "%kt #p_kS'".
     iPoseProof (public_sym_keyE with "[//] p_kS'") as ">sym".
     by iApply "sec". }
-  iPoseProof (initE with "ctx p_t") as "{p_t} [contra|p_t]".
-    by iDestruct ("sec" with "contra") as ">[]".
-  iModIntro. iDestruct "p_t" as "(%ok & #done' & frag)".
+  iDestruct "p_t" as "[p_t|p_t]".
+    by iDestruct ("sec" with "p_t") as ">[]".
+  iModIntro. iDestruct "p_t" as "(%ok & %γ & #done' & frag)".
   iPoseProof (handshake_done_session_key with "done' key") as "->".
-  by rewrite e_ok. }
+  rewrite e_ok.
+  iExists γ. eauto. }
 wp_pures.
 iApply (wp_server_conn_handler _ ss with "[#] [#] [$]") => //.
 by iIntros "!> % []".
